examples/doublylinkedlist/DoublyLinkedListIface.fst
@@ -1,0 +1,1040 @@
+(*
+   Copyright 2008-2019 Microsoft Research
+
+   Licensed under the Apache License, Version 2.0 (the "License");
+   you may not use this file except in compliance with the License.
+   You may obtain a copy of the License at
+
+       http://www.apache.org/licenses/LICENSE-2.0
+
+   Unless required by applicable law or agreed to in writing, software
+   distributed under the License is distributed on an "AS IS" BASIS,
+   WITHOUT WARRANTIES OR CONDITIONS OF ANY KIND, either express or implied.
+   See the License for the specific language governing permissions and
+   limitations under the License.
+*)
+
+module DoublyLinkedListIface
+
+/// This module consists of proofs / code for the iface that is
+/// written in the actual fsti. Most of this code will never be user
+/// facing, and will soon be merged into the DoublyLinkedList module,
+/// as I work on moving stuff into DoublLinkedList.fsti from the iface
+/// fsti.
+
+module DLL = DoublyLinkedList
+
+module HS = FStar.HyperStack
+module HST = FStar.HyperStack.ST
+module G = FStar.Ghost
+module L = FStar.List.Pure
+module B = LowStar.Buffer
+
+open LowStar.BufferOps
+
+/// Convenience operators
+
+unfold let (@) (a:B.pointer 't) (h0:HS.mem) = B.get h0 a 0
+unfold let (^@) (a:B.pointer_or_null 't{a =!= B.null}) (h0:HS.mem) = B.get h0 a 0
+
+/// Abstract types defined by this library
+///
+/// Note: Somehow confusingly, a node in the iface is a pointer to a
+/// real node, and a dll in the iface is a pointer to a real
+/// dll. Fortunately though, most users of the library will never even
+/// be looking inside the implementation, and thus hopefully it won't
+/// be confusing.
+
+let node a = B.pointer (DLL.node a)
+let dll a = B.pointer (DLL.dll a)
+
+/// Abstract Validity Predicates
+
+let node_valid h n = True /\ B.live h n // XXX: why do I need the True here?
+
+let dll_valid h d =
+  B.live h d /\
+  DLL.dll_valid h (d@h) /\
+  B.loc_buffer d `B.loc_disjoint` DLL.dll_fp0 (d@h)
+
+/// Abstract node and list footprints
+
+let fp_node n = B.loc_buffer n
+
+let fp_dll h d =
+  B.loc_union (B.loc_buffer d) (DLL.dll_fp0 (d@h))
+
+/// Getters and setters for [node]s
+
+let g_node_val h n =
+  (n@h).DLL.p
+
+let node_val n =
+  (!*n).DLL.p
+
+let node_of v =
+  B.alloca (DLL.empty_node v) 1ul
+
+/// Abstract Predicate to help "recall" that updating the payload
+/// leaves connections unchanged
+
+let unchanged_node_connections h0 h1 n =
+  (n@h0).DLL.flink == (n@h1).DLL.flink /\
+  (n@h0).DLL.blink == (n@h1).DLL.blink
+
+/// Be able to modify the payload of a node easily, without affecting
+/// membership
+
+let node_update n v =
+  n *= { !*n with DLL.p = v }
+
+/// Abstract Predicate to help "recall" that [g_node_val] remains
+/// unchanged for nodes, across multiple [mem]s
+
+let unchanged_node_val (h0 h1:HS.mem) (n:node 'a) : GTot prop =
+  (B.live h0 n ==>
+   (g_node_val h0 n == g_node_val h1 n /\ B.live h1 n))
+
+let rec unchanged_node_vals (h0 h1:HS.mem) (ns:list (node 'a)) : GTot prop =
+  match ns with
+  | [] -> True
+  | n :: ns' -> unchanged_node_val h0 h1 n /\ unchanged_node_vals h0 h1 ns'
+
+/// Viewing ghostly state of a list
+
+let as_list h d =
+  G.reveal (d@h).DLL.nodes
+
+/// Creating an empty DoublyLinkedList, and quickly accessing the head
+/// and tail of a DoublyLinkedList
+
+let dll_new () =
+  B.alloca DLL.empty_list 1ul
+
+let is_empty d =
+  B.is_null (!*d).DLL.lhead
+
+let dll_head d =
+  (!*d).DLL.lhead
+
+let dll_tail d =
+  let h0 = HST.get () in
+  L.lemma_unsnoc_is_last (as_list h0 d);
+  (!*d).DLL.ltail
+
+/// Useful auxiliary lemmas
+
+(** If a node is inside a valid list, then the node is valid. *)
+val lemma_node_in_valid_dll_is_valid (h:HS.mem) (d:dll 'a) (n:node 'a) :
+  Lemma
+    (requires (dll_valid h d /\ n `L.memP` as_list h d))
+    (ensures (node_valid h n))
+let lemma_node_in_valid_dll_is_valid h d n =
+  let pos = L.index_of (as_list h d) n in
+  DLL.extract_nodelist_contained h (as_list h d) pos
+
+(** Aux lemma *)
+val _lemma_nodelist_contained_in_unmodified_mem (h0 h1:HS.mem) (s:B.loc) (nl:list (node 'a)) :
+  Lemma
+    (requires (B.modifies s h0 h1 /\
+               B.loc_disjoint s (DLL.nodelist_fp0 nl) /\
+              (DLL.nodelist_contained0 h0 nl)))
+    (ensures (DLL.nodelist_contained0 h1 nl))
+let rec _lemma_nodelist_contained_in_unmodified_mem h0 h1 s nl =
+  match nl with
+  | [] -> ()
+  | n :: ns ->
+    _lemma_nodelist_contained_in_unmodified_mem h0 h1 s ns
+
+(** Aux lemma *)
+val _lemma_nodelist_conn_in_unmodified_mem (h0 h1:HS.mem) (s:B.loc) (nl:list (node 'a)) :
+  Lemma
+    (requires (B.modifies s h0 h1 /\
+               B.loc_disjoint s (DLL.nodelist_fp0 nl) /\
+               DLL.nodelist_contained0 h0 nl /\
+              (DLL.nodelist_conn h0 nl)))
+    (ensures (DLL.nodelist_conn h1 nl))
+let rec _lemma_nodelist_conn_in_unmodified_mem h0 h1 s nl =
+  match nl with
+  | [] -> ()
+  | n1 :: rest -> match rest with
+    | [] -> ()
+    | n2 :: ns ->
+      _lemma_nodelist_conn_in_unmodified_mem h0 h1 s rest
+
+(** Aux lemma *)
+val _lemma_nodelist_disjoint_in_push (h0 h1:HS.mem) (nl:list (node 'a)) :
+  Lemma
+    (requires (HS.fresh_frame h0 h1 /\
+               DLL.nodelist_contained0 h0 nl))
+    (ensures (DLL.nodelist_fp0 nl `B.loc_disjoint` (B.loc_region_only false (HS.get_tip h1))))
+let rec _lemma_nodelist_disjoint_in_push h0 h1 nl =
+  match nl with
+  | [] -> ()
+  | n :: ns ->
+    _lemma_nodelist_disjoint_in_push h0 h1 ns
+
+(** If a new frame is pushed, then a dll remains valid and unchanged. *)
+val _auto_dll_valid_and_unchanged_through_push (h0 h1:HS.mem) (d:dll 'a) :
+  Lemma
+    (requires (dll_valid h0 d /\ HS.fresh_frame h0 h1))
+    (ensures (dll_valid h1 d /\ d@h0 == d@h1))
+    [SMTPat (dll_valid h0 d);
+     SMTPat (HS.fresh_frame h0 h1)]
+let _auto_dll_valid_and_unchanged_through_push h0 h1 d =
+  B.fresh_frame_modifies h0 h1;
+  _lemma_nodelist_contained_in_unmodified_mem h0 h1 B.loc_none (as_list h1 d);
+  _lemma_nodelist_conn_in_unmodified_mem h0 h1 B.loc_none (as_list h1 d)
+
+(** If a frame is popped, then a dll remains valid and unchanged. *)
+val _lemma_dll_valid_and_unchanged_through_pop (h0 h1:HS.mem) (d:dll 'a) :
+  Lemma
+    (requires (dll_valid h0 d /\ HS.popped h0 h1 /\
+              B.loc_disjoint (fp_dll h0 d) (B.loc_region_only false (HS.get_tip h0))))
+    (ensures (dll_valid h1 d /\ d@h0 == d@h1))
+let _lemma_dll_valid_and_unchanged_through_pop h0 h1 d =
+  B.popped_modifies h0 h1;
+  assert (B.loc_region_only false (HS.get_tip h0) `B.loc_includes`
+            B.loc_region_only false (HS.get_tip h0)); // OBSERVE
+  let loc = B.loc_region_only false (HS.get_tip h0) in
+  _lemma_nodelist_contained_in_unmodified_mem h0 h1 loc (as_list h1 d);
+  _lemma_nodelist_conn_in_unmodified_mem h0 h1 loc (as_list h1 d)
+
+(** If stack discipline is followed, then a valid modification inside
+    a push-pop pair is also valid outside of it. *)
+val _auto_dll_modified_with_push_pop (h0 h1:HS.mem) (d:dll 'a) (h2 h3:HS.mem) :
+  Lemma
+    (requires (dll_valid h0 d /\
+               HS.fresh_frame h0 h1 /\
+               B.modifies (B.loc_union (fp_dll h0 d) (fp_dll h3 d)) h1 h2 /\
+               B.loc_disjoint (fp_dll h0 d) (B.loc_region_only false (HS.get_tip h2)) /\
+               B.loc_disjoint (fp_dll h3 d) (B.loc_region_only false (HS.get_tip h2)) /\
+               HS.get_tip h1 == HS.get_tip h2 /\
+               dll_valid h2 d /\
+               HS.popped h2 h3))
+    (ensures (dll_valid h3 d))
+    [SMTPat (HS.fresh_frame h0 h1);
+     SMTPat (HS.popped h2 h3);
+     SMTPat (dll_valid h3 d)]
+let _auto_dll_modified_with_push_pop h0 h1 d h2 h3 =
+  let loc = B.loc_region_only false (HS.get_tip h2) in
+  B.popped_modifies h2 h3;
+  _lemma_nodelist_contained_in_unmodified_mem h2 h3 loc (as_list h3 d);
+  _lemma_nodelist_conn_in_unmodified_mem h2 h3 loc (as_list h3 d)
+
+(** If a new frame is pushed, the the dll's fp is disjoint from what just got pushed. *)
+val _auto_dll_fp_disjoint_from_push (h0 h1:HS.mem) (d:dll 'a) :
+  Lemma
+    (requires (dll_valid h0 d /\ HS.fresh_frame h0 h1))
+    (ensures (B.loc_disjoint (fp_dll h0 d) (B.loc_region_only false (HS.get_tip h1))))
+    [SMTPat (dll_valid h0 d);
+     SMTPat (HS.fresh_frame h0 h1)]
+let _auto_dll_fp_disjoint_from_push h0 h1 d =
+  _lemma_nodelist_disjoint_in_push h0 h1 (G.reveal (d@h0).DLL.nodes)
+
+(** If a valid dll is placed into a pointer, it stays valid *)
+val _auto_dll_assign_valid_stays_valid (h0 h1:HS.mem) (d:dll 'a) (d2:DLL.dll 'a) :
+  Lemma
+    (requires (DLL.dll_valid h0 d2 /\
+               B.modifies (B.loc_buffer d) h0 h1 /\
+               B.loc_buffer d `B.loc_disjoint` DLL.dll_fp0 d2 /\
+               B.live h0 d /\
+               d@h1 == d2))
+    (ensures (dll_valid h1 d))
+    [SMTPat (DLL.dll_valid h0 d2);
+     SMTPat (B.modifies (B.loc_buffer d) h0 h1);
+     SMTPat (dll_valid h1 d)]
+let _auto_dll_assign_valid_stays_valid h0 h1 d d2 =
+  _lemma_nodelist_conn_in_unmodified_mem h0 h1 (B.loc_buffer d) (G.reveal d2.DLL.nodes);
+  _lemma_nodelist_contained_in_unmodified_mem h0 h1 (B.loc_buffer d) (G.reveal d2.DLL.nodes)
+
+(** [unchanged_node_vals] is transitive *)
+let rec _lemma_unchanged_node_vals_transitive (h0 h1 h2:HS.mem) (ns:list (node 'a)) :
+  Lemma
+    (requires (
+        (unchanged_node_vals h0 h1 ns) /\
+        (unchanged_node_vals h1 h2 ns)))
+    (ensures (
+        (unchanged_node_vals h0 h2 ns))) =
+  match ns with
+  | [] -> ()
+  | _ :: ns' -> _lemma_unchanged_node_vals_transitive h0 h1 h2 ns'
+
+(** Auxiliary predicate: node list is disjoint from region *)
+let rec _pred_nl_disjoint (h:HS.mem) (ns:list (node 'a)) =
+  DLL.nodelist_fp0 ns `B.loc_disjoint` B.loc_region_only false (HS.get_tip h)
+
+(** If [unchanged_node_vals] is true, then it remains true through a push-pop. *)
+val _auto_unchanged_node_vals_through_push_pop (h0 h1:HS.mem) (ns:list (node 'a)) (h2 h3:HS.mem) :
+  Lemma
+    (requires (unchanged_node_vals h1 h2 ns /\
+               HS.fresh_frame h0 h1 /\ HS.popped h2 h3 /\
+               _pred_nl_disjoint h1 ns /\
+               HS.get_tip h1 == HS.get_tip h2))
+    (ensures (
+        unchanged_node_vals h0 h1 ns /\ // used only for proof. not necessary outside
+        unchanged_node_vals h2 h3 ns /\ // used only for proof. not necessary outside
+        unchanged_node_vals h0 h3 ns))
+    [SMTPat (unchanged_node_vals h0 h3 ns);
+     SMTPat (HS.fresh_frame h0 h1);
+     SMTPat (HS.popped h2 h3)]
+let rec _auto_unchanged_node_vals_through_push_pop h0 h1 ns h2 h3 =
+  match ns with
+  | [] -> ()
+  | n :: ns' ->
+    _auto_unchanged_node_vals_through_push_pop h0 h1 ns' h2 h3;
+    // assert (unchanged_node_vals h0 h1 ns);
+    // assert (unchanged_node_vals h2 h3 ns);
+    B.popped_modifies h2 h3
+
+(** If a valid dll has a frame pushed, [_pred_nl_disjoint] stays true *)
+val _auto_pred_nl_disjoint_push (h0 h1:HS.mem) (d:dll 'a) :
+  Lemma
+    (requires (dll_valid h0 d /\ HS.fresh_frame h0 h1))
+    (ensures (_pred_nl_disjoint h1 (as_list h1 d)))
+    [SMTPat (dll_valid h0 d);
+     SMTPat (HS.fresh_frame h0 h1)]
+let _auto_pred_nl_disjoint_push h0 h1 d =
+  let loc = B.loc_region_only false (HS.get_tip h1) in
+  let rec aux (ns:list (node 'a)) :
+    Lemma
+      (requires (DLL.nodelist_contained h0 ns /\ HS.fresh_frame h0 h1))
+      (ensures (_pred_nl_disjoint h1 ns)) =
+    match ns with
+    | [] -> ()
+    | n :: ns' -> aux ns'
+  in
+  aux (as_list h0 d)
+
+(** The impl version of [unchanged_node_vals] is same as iface one *)
+let rec _auto_unchanged_node_vals_DLL (h0 h1:HS.mem) (ns:list (node 'a)) :
+  Lemma
+    (requires (DLL.unchanged_node_vals h0 h1 ns))
+    (ensures (unchanged_node_vals h0 h1 ns))
+    [SMTPat (unchanged_node_vals h0 h1 ns)] =
+  match ns with
+  | [] -> ()
+  | _ :: ns' -> _auto_unchanged_node_vals_DLL h0 h1 ns'
+
+(** If a valid dll is placed into a pointer, its nodes stay unchanged *)
+val _auto_unchanged_node_vals_stays_valid (h0 h1:HS.mem) (d:dll 'a) (d2:DLL.dll 'a) :
+  Lemma
+    (requires (DLL.dll_valid h0 d2 /\
+               B.modifies (B.loc_buffer d) h0 h1 /\
+               B.loc_buffer d `B.loc_disjoint` DLL.dll_fp0 d2 /\
+               B.live h0 d /\
+               d@h1 == d2))
+    (ensures (unchanged_node_vals h0 h1 (as_list h1 d)))
+    [SMTPat (DLL.dll_valid h0 d2);
+     SMTPat (B.modifies (B.loc_buffer d) h0 h1);
+     SMTPat (unchanged_node_vals h0 h1 (as_list h1 d))]
+let _auto_unchanged_node_vals_stays_valid h0 h1 d d2 =
+  let rec aux nl : Lemma
+    (requires (
+       B.modifies (B.loc_buffer d) h0 h1 /\
+       DLL.nodelist_fp0 nl `B.loc_disjoint` B.loc_buffer d))
+    (ensures (unchanged_node_vals h0 h1 nl)) =
+    match nl with
+    | [] -> ()
+    | n :: ns -> aux ns in
+  aux (as_list h1 d)
+
+(** If a nodelist is disjoint from a modification, it stays unchanged *)
+let rec _lemma_unchanged_node_vals_when_disjoint (h0 h1:HS.mem) loc nl : Lemma
+    (requires (
+        B.modifies loc h0 h1 /\
+        DLL.nodelist_fp0 nl `B.loc_disjoint` loc))
+    (ensures (unchanged_node_vals h0 h1 nl)) =
+  match nl with
+  | [] -> ()
+  | n :: ns -> _lemma_unchanged_node_vals_when_disjoint h0 h1 loc ns
+
+(** If a dll is assigned to, its original nodes stay unchanged *)
+val _lemma_unchanged_node_vals_stays_valid0 (h0 h1:HS.mem) (d:dll 'a) :
+  Lemma
+    (requires (B.modifies (B.loc_buffer d) h0 h1 /\
+               B.loc_buffer d `B.loc_disjoint` DLL.dll_fp0 (d@h0) /\
+               B.live h0 d))
+    (ensures (unchanged_node_vals h0 h1 (as_list h0 d)))
+let _lemma_unchanged_node_vals_stays_valid0 h0 h1 d =
+  _lemma_unchanged_node_vals_when_disjoint h0 h1 (B.loc_buffer d) (as_list h0 d)
+
+(** If a node belongs to a dll, then its fp is included *)
+let rec _lemma_node_in_list_is_included (n:node 'a) (nl:list (node 'a)) :
+  Lemma
+    (requires (n `L.memP` nl))
+    (ensures (DLL.nodelist_fp0 nl `B.loc_includes` fp_node n)) =
+  match nl with
+  | [_] -> ()
+  | n' :: ns ->
+    FStar.Classical.or_elim #_ #_ #(fun () -> DLL.nodelist_fp0 nl `B.loc_includes` fp_node n)
+      (fun (_:unit{n == n'}) -> ())
+      (fun (_:unit{n =!= n'}) -> _lemma_node_in_list_is_included n ns)
+
+(** If a node_or_null is null or belongs to a dll, then its fp is included *)
+let _lemma_node_in_list_or_null_is_included (n:B.pointer_or_null (DLL.node 'a)) (nl:list (node 'a)) :
+  Lemma
+    (requires (n =!= B.null ==> n `L.memP` nl))
+    (ensures (DLL.nodelist_fp0 nl `B.loc_includes` B.loc_buffer n)) =
+  FStar.Classical.arrow_to_impl
+  #(n =!= B.null) #(DLL.nodelist_fp0 nl `B.loc_includes` B.loc_buffer n)
+    (fun _ -> _lemma_node_in_list_is_included n nl)
+
+(** If a node is in the list, then the node before it is also in the list if it is not null *)
+let _lemma_prev_node_in_list (h:HS.mem) (n:node 'a) (d:dll 'a) :
+  Lemma
+    (requires (dll_valid h d /\ n `L.memP` as_list h d))
+    (ensures (let n' = (n@h).DLL.blink in
+              n' =!= B.null ==> n' `L.memP` as_list h d)) =
+  let n' = (n@h).DLL.blink in
+  let l = as_list h d in
+  FStar.Classical.arrow_to_impl
+  #(n' =!= B.null) #(n' =!= B.null /\ n' `L.memP` l)
+  (fun _ ->
+    lemma_node_in_valid_dll_is_valid h d n;
+    DLL.extract_nodelist_conn h l (L.index_of l n - 1))
+
+(** If a node is in the list, then the node after it is also in the list if it is not null *)
+let _lemma_next_node_in_list (h:HS.mem) (n:node 'a) (d:dll 'a) :
+  Lemma
+    (requires (dll_valid h d /\ n `L.memP` as_list h d))
+    (ensures (let n' = (n@h).DLL.flink in
+              n' =!= B.null ==> n' `L.memP` as_list h d)) =
+  let n' = (n@h).DLL.flink in
+  let l = as_list h d in
+  FStar.Classical.arrow_to_impl
+  #(n' =!= B.null) #(n' =!= B.null /\ n' `L.memP` l)
+  (fun _ ->
+    lemma_node_in_valid_dll_is_valid h d n;
+    L.lemma_unsnoc_is_last l;
+    DLL.extract_nodelist_conn h l (L.index_of l n))
+
+(** Insertion operations maintain membership *)
+let rec _lemma_insertion_maintains_memP (l1 l2:list 'a) (x0 x1 x:'a) :
+  Lemma
+    (requires ((x0 `L.memP` l1) /\
+               ((l2 == DLL._l_insert_before x0 l1 x1) \/
+                (l2 == DLL._l_insert_after x0 l1 x1)) /\
+               (x `L.memP` l1 \/ x == x1)))
+    (ensures (x `L.memP` l2)) =
+  match l1 with
+  | [_] -> ()
+  | x0' :: l1' ->
+    FStar.Classical.or_elim #_ #_ #(fun () -> x `L.memP` l2)
+      (fun (_:unit{x0' == x0 \/ x0' == x}) -> ())
+      (fun (_:unit{x0' =!= x0 /\ x0' =!= x}) ->
+         _lemma_insertion_maintains_memP l1' (L.tl l2) x0 x1 x)
+
+(** Insertion operations maintain [unchanged_node_vals] *)
+let rec _lemma_insertion_maintains_unchanged_node_vals (h0 h1:HS.mem) (l1 l2:list (node 'a)) (x0 x1:node 'a) :
+  Lemma
+    (requires ((x0 `L.memP` l1) /\
+               ((l2 == DLL._l_insert_before x0 l1 x1) \/
+                (l2 == DLL._l_insert_after x0 l1 x1)) /\
+               (unchanged_node_vals h0 h1 l2)))
+    (ensures (unchanged_node_vals h0 h1 l1)) =
+  match l1 with
+  | [_] -> ()
+  | x0' :: l1' ->
+    FStar.Classical.arrow_to_impl #(x0 =!= x0') #(unchanged_node_vals h0 h1 l1)
+      (fun _ ->
+         _lemma_insertion_maintains_unchanged_node_vals h0 h1 l1' (L.tl l2) x0 x1)
+
+(** Unchanged node vals means that the payloads maintain the changes
+    that happened *)
+let rec _lemma_unchanged_node_vals_maintains_changes (h0 h1:HS.mem) (l:list (node 'a)) :
+  Lemma
+    (requires (DLL.nodelist_contained h0 l /\ unchanged_node_vals h0 h1 l))
+    (ensures (g_node_vals h1 l == g_node_vals h0 l)) =
+  match l with
+  | [] -> ()
+  | h :: t ->
+    _lemma_unchanged_node_vals_maintains_changes h0 h1 t
+
+(** Containment holds before/after [append]ing *)
+let rec _lemma_append_contains (h0:HS.mem) (l1 l2:list (node 'a)) :
+  Lemma
+    (ensures (
+        (DLL.nodelist_contained h0 (l1 `L.append` l2)) <==>
+        (DLL.nodelist_contained h0 l1 /\ DLL.nodelist_contained h0 l2))) =
+  match l1 with
+  | [] -> ()
+  | h :: t -> _lemma_append_contains h0 t l2
+
+(** [g_node_vals] before/after [append]ing *)
+let rec _lemma_append_g_node_vals (h0:HS.mem) (l1 l2:list (node 'a)) :
+  Lemma
+    (ensures (
+        (g_node_vals h0 (l1 `L.append` l2) == g_node_vals h0 l1 `L.append` g_node_vals h0 l2))) =
+  match l1 with
+  | [] -> ()
+  | h :: t -> _lemma_append_g_node_vals h0 t l2
+
+(** [unchanged_node_val] before/after [append]ing *)
+let rec _lemma_unchanged_node_vals_append (h0 h1:HS.mem) (l1 l2:list (node 'a)) :
+  Lemma
+    (ensures (
+        (unchanged_node_vals h0 h1 (l1 `L.append` l2) <==>
+         (unchanged_node_vals h0 h1 l1 /\ unchanged_node_vals h0 h1 l2)))) =
+  match l1 with
+  | [] -> ()
+  | h :: t -> _lemma_unchanged_node_vals_append h0 h1 t l2
+
+(** Getting a specific node from an [unchanged_node_val] *)
+let rec _lemma_extract_unchanged_node_val (h0 h1:HS.mem) (n:node 'a) (l:list (node 'a)) :
+  Lemma
+    (requires (unchanged_node_vals h0 h1 l /\ n `L.memP` l))
+    (ensures (unchanged_node_val h0 h1 n)) =
+  let h :: t = l in
+  FStar.Classical.or_elim #_ #_ #(fun () -> unchanged_node_val h0 h1 n)
+    (fun (_:unit{n == h}) -> ())
+    (fun (_:unit{n =!= h}) -> _lemma_extract_unchanged_node_val h0 h1 n t)
+
+(** Connect [split_using] and [splitAt] *)
+let rec _lemma_split_using_splitAt (l:list 'a) (x:'a) :
+  Lemma
+    (requires (x `L.memP` l))
+    (ensures
+       (l `L.split_using` x == L.splitAt (l `L.index_of` x) l)) =
+  match l with
+  | [_] -> ()
+  | h :: t ->
+    FStar.Classical.arrow_to_impl
+    #(x `L.memP` t)
+    #(l `L.split_using` x == L.splitAt (l `L.index_of` x) l)
+      (fun _ -> _lemma_split_using_splitAt t x)
+
+(** Length of a [g_node_vals] is same as orig list *)
+let rec _lemma_length_g_node_vals (h0:HS.mem) (l:list (node 'a)) :
+  Lemma
+    (L.length (g_node_vals h0 l) = L.length l) =
+  match l with
+  | [] -> ()
+  | h :: t ->
+    _lemma_length_g_node_vals h0 t
+
+/// Moving forwards or backwards in a list
+
+let has_next d n =
+  let h0 = HST.get () in
+  DLL.lemma_dll_links_contained h0 (d@h0) (as_list h0 d `L.index_of` n);
+  L.lemma_unsnoc_is_last (as_list h0 d);
+  let y = not (B.is_null (!*n).DLL.flink) in
+  FStar.Classical.or_elim #_ #_ #(fun () ->
+      y <==> as_list h0 d `L.index_of` n < L.length (as_list h0 d) - 1)
+    (fun (_:unit{y}) -> ())
+    (fun (_:unit{not y}) ->
+       DLL._lemma_only_tail_can_point_right_to_null h0 n (as_list h0 d);
+       DLL._lemma_all_nodes_are_unique h0 (as_list h0 d)
+         (as_list h0 d `L.index_of` n)
+         (L.length (as_list h0 d) - 1));
+  y
+
+let has_prev d n =
+  let h0 = HST.get () in
+  DLL.lemma_dll_links_contained h0 (d@h0) (as_list h0 d `L.index_of` n);
+  L.lemma_unsnoc_is_last (as_list h0 d);
+  let y = not (B.is_null (!*n).DLL.blink) in
+  FStar.Classical.or_elim #_ #_ #(fun () ->
+      y <==> as_list h0 d `L.index_of` n > 0)
+    (fun (_:unit{y}) -> ())
+    (fun (_:unit{not y}) ->
+       DLL._lemma_only_head_can_point_left_to_null h0 n (as_list h0 d);
+       DLL._lemma_all_nodes_are_unique h0 (as_list h0 d)
+         (as_list h0 d `L.index_of` n)
+         0);
+  y
+
+let next_node d n =
+  let h0 = HST.get () in
+  lemma_node_in_valid_dll_is_valid h0 d n;
+  DLL.extract_nodelist_conn h0 (as_list h0 d) (L.index_of (as_list h0 d) n);
+  (!*n).DLL.flink
+
+let prev_node d n =
+  let h0 = HST.get () in
+  lemma_node_in_valid_dll_is_valid h0 d n;
+  DLL.extract_nodelist_conn h0 (as_list h0 d) (L.index_of (as_list h0 d) n - 1);
+  (!*n).DLL.blink
+
+/// Stateful DoublyLinkedList operations
+///
+/// These are most likely what you want to be using when writing
+/// code. The rest of this interface lets you talk about these
+/// operations easily.
+
+#set-options "--z3rlimit 20 --max_fuel 2 --max_ifuel 1"
+
+let dll_insert_at_head #t d n =
+  let h00 = HST.get () in
+  HST.push_frame ();
+  let h0 = HST.get () in
+  let y = DLL.dll_insert_at_head (!*d) n in
+  let h' = HST.get () in
+  d *= y;
+  let h1 = HST.get () in
+  _lemma_unchanged_node_vals_transitive h0 h' h1 (as_list h1 d);
+  HST.pop_frame ();
+  let h11 = HST.get () in
+  _lemma_unchanged_node_vals_maintains_changes h00 h11 (as_list h1 d)
+
+#reset-options
+
+#set-options "--z3rlimit 40 --max_fuel 2 --max_ifuel 1"
+
+let dll_insert_at_tail #t d n =
+  let h00 = HST.get () in
+  HST.push_frame ();
+  let h0 = HST.get () in
+  let y = DLL.dll_insert_at_tail (!*d) n in
+  let h' = HST.get () in
+  d *= y;
+  let h1 = HST.get () in
+  assert (_pred_nl_disjoint h0 (as_list h1 d)); // OBSERVE
+  _lemma_unchanged_node_vals_transitive h0 h' h1 (as_list h1 d);
+  HST.pop_frame ();
+  let h11 = HST.get () in
+  _lemma_append_contains h00 (as_list h0 d) [n];
+  _lemma_unchanged_node_vals_maintains_changes h00 h11 (as_list h1 d);
+  _lemma_append_g_node_vals h11 (as_list h0 d) [n];
+  L.lemma_unsnoc_is_last (as_list h1 d);
+  _lemma_extract_unchanged_node_val h0 h1 n (as_list h1 d);
+  _lemma_append_g_node_vals h00 (as_list h0 d) [n];
+  _lemma_unchanged_node_vals_append h00 h11 (as_list h0 d) [n]
+
+#reset-options
+
+#set-options "--z3rlimit 80 --max_fuel 2 --max_ifuel 1"
+
+let dll_insert_before #t n' d n =
+  let h00 = HST.get () in
+  HST.push_frame ();
+  let h0 = HST.get () in
+  let y = DLL.dll_insert_before (!*d) n' n in
+  let h' = HST.get () in
+  d *= y;
+  let h1 = HST.get () in
+  assert (_pred_nl_disjoint h0 (as_list h1 d)); // OBSERVE
+  _lemma_unchanged_node_vals_transitive h0 h' h1 (as_list h1 d);
+  // assert (fp_dll h1 d `B.loc_includes` (B.loc_buffer (d@h0).DLL.lhead));
+  // assert (fp_dll h1 d `B.loc_includes` (B.loc_buffer (d@h0).DLL.ltail));
+  // assert (fp_dll h1 d `B.loc_includes` (B.loc_buffer n));
+  _lemma_insertion_maintains_memP (as_list h0 d) (as_list h1 d) n' n n';
+  // assert (n' `L.memP` as_list h1 d);
+  _lemma_prev_node_in_list h0 n' d;
+  FStar.Classical.arrow_to_impl #((n'@h0).DLL.blink =!= B.null)
+    #((n'@h0).DLL.blink =!= B.null /\ (n'@h0).DLL.blink `L.memP` as_list h1 d)
+    (fun _ ->
+       _lemma_insertion_maintains_memP (as_list h0 d) (as_list h1 d) n' n (n'@h0).DLL.blink);
+  // assert ((n'@h0).DLL.blink =!= B.null ==> (n'@h0).DLL.blink `L.memP` as_list h1 d);
+  _lemma_node_in_list_is_included n' (as_list h1 d);
+  _lemma_node_in_list_or_null_is_included (n'@h0).DLL.blink (as_list h1 d);
+  // assert (fp_dll h1 d `B.loc_includes` (B.loc_buffer n'));
+  // assert (fp_dll h1 d `B.loc_includes` (B.loc_buffer (n'@h0).DLL.blink));
+  // assert (B.modifies (fp_dll h1 d) h0 h1);
+  HST.pop_frame ();
+  let h11 = HST.get () in
+  _lemma_split_using_splitAt (as_list h00 d) n';
+  _lemma_append_g_node_vals h11
+    (fst (L.splitAt (as_list h00 d `L.index_of` n') (as_list h00 d)))
+    (snd (L.splitAt (as_list h00 d `L.index_of` n') (as_list h00 d)));
+  L.lemma_splitAt_append (as_list h00 d `L.index_of` n') (as_list h00 d);
+  _lemma_length_g_node_vals h00 (as_list h00 d);
+  L.lemma_splitAt_append (as_list h00 d `L.index_of` n') (g_node_vals h00 (as_list h00 d));
+  // assert ((as_list h00 d `L.index_of` n') < L.length (g_node_vals h00 (as_list h00 d)));
+  _lemma_insertion_maintains_unchanged_node_vals h0 h1 (as_list h0 d) (as_list h1 d) n' n;
+  // assert (unchanged_node_vals h0 h1 (as_list h0 d));
+  _lemma_unchanged_node_vals_maintains_changes h00 h11 (as_list h00 d);
+  // assert (g_node_vals h11 (as_list h00 d) == g_node_vals h00 (as_list h00 d));
+  // assert (
+  //   let l1, l2 = L.splitAt (as_list h00 d `L.index_of` n') (as_list h00 d) in
+  //   let m1, m2 = L.splitAt (as_list h00 d `L.index_of` n') (g_node_vals h00 (as_list h00 d)) in
+  //   g_node_vals h11
+  //     (l1 `L.append` l2) == (m1 `L.append` m2) /\ L.length l1 = L.length m1);
+  L.lemma_splitAt_append (as_list h00 d `L.index_of` n') (g_node_vals h00 (as_list h00 d));
+  _lemma_length_g_node_vals h11 (fst (L.splitAt (as_list h00 d `L.index_of` n') (as_list h00 d)));
+  L.append_length_inv_head
+    (g_node_vals h11 (fst (L.splitAt (as_list h00 d `L.index_of` n') (as_list h00 d))))
+    (g_node_vals h11 (snd (L.splitAt (as_list h00 d `L.index_of` n') (as_list h00 d))))
+    (fst (L.splitAt (as_list h00 d `L.index_of` n') (g_node_vals h00 (as_list h00 d))))
+    (snd (L.splitAt (as_list h00 d `L.index_of` n') (g_node_vals h00 (as_list h00 d))));
+  // assert (g_node_vals h11 (let l1, l2 = L.splitAt (as_list h00 d `L.index_of` n') (as_list h00 d) in l1) == (
+  //     let l1, l2 = L.splitAt (as_list h00 d `L.index_of` n') (g_node_vals h00 (as_list h00 d)) in
+  //     l1));
+  // assert (g_node_vals h11 (let l1, l2 = L.splitAt (as_list h00 d `L.index_of` n') (as_list h00 d) in l2) == (
+  //     let l1, l2 = L.splitAt (as_list h00 d `L.index_of` n') (g_node_vals h00 (as_list h00 d)) in
+  //     l2));
+  // assert (g_node_vals h11 (let l1, l2 = L.split_using (as_list h00 d) n' in l1) == (
+  //     let l1, l2 = L.splitAt (as_list h00 d `L.index_of` n') (g_node_vals h00 (as_list h00 d)) in
+  //     l1));
+  // assert (g_node_vals h11 (let l1, l2 = L.split_using (as_list h00 d) n' in l2) == (
+  //     let l1, l2 = L.splitAt (as_list h00 d `L.index_of` n') (g_node_vals h00 (as_list h00 d)) in
+  //     l2));
+  _lemma_insertion_maintains_memP (as_list h0 d) (as_list h1 d) n' n n;
+  // assert (n `L.memP` as_list h1 d);
+  _lemma_extract_unchanged_node_val h0 h1 n (as_list h1 d);
+  // assert (g_node_val h1 n == g_node_val h0 n);
+  _lemma_append_g_node_vals h11
+    (let l1, l2 = L.split_using (as_list h00 d) n' in l1)
+    (let l1, l2 = L.split_using (as_list h00 d) n' in (n :: l2));
+  // assert (g_node_vals h11 (
+  //     let l1, l2 = L.split_using (as_list h00 d) n' in
+  //     l1 `L.append` (n :: l2)) == (
+  //     let l1, l2 = L.splitAt (as_list h00 d `L.index_of` n') (g_node_vals h00 (as_list h00 d)) in
+  //     l1 `L.append` ((g_node_val h00 n) :: l2)));
+  // assert (g_node_vals h11 (l_insert_before n' (as_list h00 d) n) == (
+  //     let l1, l2 = L.splitAt (as_list h00 d `L.index_of` n') (g_node_vals h00 (as_list h00 d)) in
+  //     l1 `L.append` ((g_node_val h00 n) :: l2)));
+  // assert (g_node_vals h11 (as_list h11 d) == (
+  //     let l1, l2 = L.splitAt (as_list h00 d `L.index_of` n') (g_node_vals h00 (as_list h00 d)) in
+  //     l1 `L.append` ((g_node_val h00 n) :: l2)));
+  // assert (as_payload_list h11 d == (
+  //     let l1, l2 = L.splitAt (as_list h00 d `L.index_of` n') (as_payload_list h00 d) in
+  //     l1 `L.append` ((g_node_val h00 n) :: l2)));
+  // assert (as_payload_list h11 d == l_insert_before'
+  //           (as_list h00 d `L.index_of` n') (as_payload_list h00 d) (g_node_val h00 n));
+  ()
+
+#reset-options
+
+#set-options "--z3rlimit 80 --max_fuel 2 --max_ifuel 1"
+
+let dll_insert_after #t n' d n =
+  let h00 = HST.get () in
+  HST.push_frame ();
+  let h0 = HST.get () in
+  let y = DLL.dll_insert_after (!*d) n' n in
+  let h' = HST.get () in
+  d *= y;
+  let h1 = HST.get () in
+  assert (_pred_nl_disjoint h0 (as_list h1 d)); // OBSERVE
+  _lemma_unchanged_node_vals_transitive h0 h' h1 (as_list h1 d);
+  _lemma_insertion_maintains_memP (as_list h0 d) (as_list h1 d) n' n n';
+  _lemma_next_node_in_list h0 n' d;
+  FStar.Classical.arrow_to_impl #((n'@h0).DLL.flink =!= B.null)
+    #((n'@h0).DLL.flink =!= B.null /\ (n'@h0).DLL.flink `L.memP` as_list h1 d)
+    (fun _ ->
+       _lemma_insertion_maintains_memP (as_list h0 d) (as_list h1 d) n' n (n'@h0).DLL.flink);
+  _lemma_node_in_list_is_included n' (as_list h1 d);
+  _lemma_node_in_list_or_null_is_included (n'@h0).DLL.flink (as_list h1 d);
+  // assert (B.modifies (fp_dll h1 d) h0 h1);
+  HST.pop_frame ();
+  let h11 = HST.get () in
+  admit () (* Due to recent "double ghost" change *)
+
+#reset-options
+
+#set-options "--z3rlimit 40 --max_fuel 2 --max_ifuel 1"
+
+let dll_remove_head #t d =
+  let h00 = HST.get () in
+  HST.push_frame ();
+  let h0 = HST.get () in
+  let y = DLL.dll_remove_head (!*d) in
+  let h' = HST.get () in
+  d *= y;
+  let h1 = HST.get () in
+  _lemma_unchanged_node_vals_stays_valid0 h' h1 d;
+  _lemma_unchanged_node_vals_transitive h0 h' h1 (as_list h0 d);
+  HST.pop_frame ();
+  let h11 = HST.get () in
+  admit () (* Due to recent "double ghost" change *)
+
+#reset-options
+
+#set-options "--z3rlimit 40 --max_fuel 2 --max_ifuel 1"
+
+let dll_remove_tail #t d =
+  let h00 = HST.get () in
+  HST.push_frame ();
+  let h0 = HST.get () in
+  let y = DLL.dll_remove_tail (!*d) in
+  let h' = HST.get () in
+  d *= y;
+  let h1 = HST.get () in
+
+  FStar.Classical.arrow_to_impl
+  #(L.length (G.reveal (d@h0).DLL.nodes) >= 2)
+  #(DLL.dll_fp0 (d@h0) `B.loc_includes` B.loc_buffer ((d@h0).DLL.ltail@h0).DLL.blink)
+    (fun _ ->
+       DLL.extract_nodelist_conn h0 (G.reveal (d@h0).DLL.nodes) (L.length (G.reveal (d@h0).DLL.nodes) - 2);
+       DLL.extract_nodelist_fp0 (G.reveal (d@h0).DLL.nodes) (L.length (G.reveal (d@h0).DLL.nodes) - 2);
+       L.lemma_unsnoc_is_last (G.reveal (d@h0).DLL.nodes));
+
+  _lemma_unchanged_node_vals_stays_valid0 h' h1 d;
+  _lemma_unchanged_node_vals_transitive h0 h' h1 (as_list h0 d);
+  HST.pop_frame ();
+  let h11 = HST.get () in
+  admit () (* Due to recent "double ghost" change *)
+
+#reset-options
+
+#set-options "--z3rlimit 40 --max_fuel 2 --max_ifuel 1"
+
+let dll_remove_mid #t d n =
+  let h00 = HST.get () in
+  HST.push_frame ();
+  let h0 = HST.get () in
+  let y = DLL.dll_remove_node (!*d) n in
+  let h' = HST.get () in
+  d *= y;
+  let h1 = HST.get () in
+
+  FStar.Classical.arrow_to_impl
+  #(L.length (G.reveal (d@h0).DLL.nodes) >= 2)
+  #(DLL.dll_fp0 (d@h0) `B.loc_includes` B.loc_buffer ((d@h0).DLL.ltail@h0).DLL.blink)
+    (fun _ ->
+       DLL.extract_nodelist_conn h0 (G.reveal (d@h0).DLL.nodes) (L.length (G.reveal (d@h0).DLL.nodes) - 2);
+       DLL.extract_nodelist_fp0 (G.reveal (d@h0).DLL.nodes) (L.length (G.reveal (d@h0).DLL.nodes) - 2);
+       L.lemma_unsnoc_is_last (G.reveal (d@h0).DLL.nodes));
+  // assert (DLL.dll_fp0 (d@h0) `B.loc_includes` B.loc_buffer ((d@h0).DLL.lhead@h0).DLL.flink);
+  // assert (DLL.dll_fp0 (d@h0) `B.loc_includes` B.loc_buffer ((d@h0).DLL.ltail@h0).DLL.blink);
+
+  _lemma_next_node_in_list h0 n d;
+  _lemma_node_in_list_or_null_is_included ((n@h0).DLL.flink) (G.reveal (d@h0).DLL.nodes);
+  _lemma_prev_node_in_list h0 n d;
+  _lemma_node_in_list_or_null_is_included ((n@h0).DLL.blink) (G.reveal (d@h0).DLL.nodes);
+  // assert (DLL.dll_fp0 (d@h0) `B.loc_includes` B.loc_buffer (n@h0).DLL.flink);
+  // assert (DLL.dll_fp0 (d@h0) `B.loc_includes` B.loc_buffer (n@h0).DLL.blink);
+
+  _lemma_unchanged_node_vals_stays_valid0 h' h1 d;
+  _lemma_unchanged_node_vals_transitive h0 h' h1 (as_list h0 d);
+  HST.pop_frame ();
+  let h11 = HST.get () in
+  admit () (* Due to recent "double ghost" change *)
+
+#reset-options
+
+#set-options "--z3rlimit 20 --max_fuel 2 --max_ifuel 1"
+
+let dll_append #t d1 d2 =
+  let h00 = HST.get () in
+  HST.push_frame ();
+  let h0 = HST.get () in
+  let y = DLL.dll_append (!*d1) (!*d2) in
+  let h' = HST.get () in
+  d1 *= y;
+  let h1 = HST.get () in
+  DLL.nodelist_append_fp0 (as_list h0 d1) (as_list h0 d2);
+  assert (_pred_nl_disjoint h0 (as_list h1 d1)); // OBSERVE
+  _lemma_unchanged_node_vals_transitive h0 h' h1 (as_list h1 d1);
+  HST.pop_frame ();
+  let h11 = HST.get () in
+  admit () (* Due to recent "double ghost" change *)
+
+#reset-options
+
+#set-options "--z3rlimit 100 --max_fuel 2 --max_ifuel 1"
+
+let dll_split_using #t d1 d2 n =
+  let h00 = HST.get () in
+  HST.push_frame ();
+  let h0 = HST.get () in
+  let y1, y2 = DLL.dll_split_using (!*d1) n in
+  let h0' = HST.get () in
+  d1 *= y1;
+  let h0'' = HST.get () in
+  d2 *= y2;
+  let h1 = HST.get () in
+  assert (B.loc_buffer d1 `B.loc_disjoint` DLL.dll_fp0 (d1@h0));
+  assert (DLL.dll_fp0 (d1@h0) `B.loc_includes` DLL.dll_fp0 y1);
+  FStar.Classical.arrow_to_impl
+  #(L.length (G.reveal (d1@h0).DLL.nodes) >= 2)
+  #(DLL.dll_fp0 (d1@h0) `B.loc_includes` B.loc_buffer ((d1@h0).DLL.ltail@h0).DLL.blink)
+    (fun _ ->
+       DLL.extract_nodelist_conn h0 (G.reveal (d1@h0).DLL.nodes) (L.length (G.reveal (d1@h0).DLL.nodes) - 2);
+       DLL.extract_nodelist_fp0 (G.reveal (d1@h0).DLL.nodes) (L.length (G.reveal (d1@h0).DLL.nodes) - 2);
+       L.lemma_unsnoc_is_last (G.reveal (d1@h0).DLL.nodes));
+  _lemma_prev_node_in_list h0 n d1;
+  _lemma_node_in_list_or_null_is_included ((n@h0).DLL.blink) (G.reveal (d1@h0).DLL.nodes);
+  _lemma_node_in_list_is_included n (G.reveal (d1@h0).DLL.nodes);
+  assert (B.loc_buffer d1 `B.loc_disjoint` DLL.dll_fp0 (d1@h0'));
+  _lemma_unchanged_node_vals_stays_valid0 h0' h0'' d1;
+  _lemma_unchanged_node_vals_transitive h0 h0' h0'' (as_list h0 d1);
+  //
+  _lemma_unchanged_node_vals_when_disjoint h0'' h1 (B.loc_buffer d2) (as_list h0 d1);
+  assert (unchanged_node_vals h0'' h1 (as_list h0 d1));
+  assert (_pred_nl_disjoint h0 (as_list h0 d1));
+  assert (_pred_nl_disjoint h0 (as_list h1 d1));
+  assert (_pred_nl_disjoint h0 (as_list h1 d2));
+  _lemma_unchanged_node_vals_transitive h0 h0'' h1 (as_list h0 d1);
+  assert (dll_valid h0'' d1);
+  _lemma_nodelist_conn_in_unmodified_mem h0'' h1 (B.loc_buffer d2) (as_list h0'' d1);
+  _lemma_nodelist_contained_in_unmodified_mem h0'' h1 (B.loc_buffer d2) (as_list h0'' d1);
+  assert (dll_valid h1 d1);
+  _lemma_nodelist_conn_in_unmodified_mem h0' h0'' (B.loc_buffer d1) (G.reveal y2.DLL.nodes);
+  _lemma_nodelist_contained_in_unmodified_mem h0' h0'' (B.loc_buffer d1) (G.reveal y2.DLL.nodes);
+  assert (DLL.dll_valid h0'' y2);
+  assert (dll_valid h1 d2);
+  HST.pop_frame ();
+  let h11 = HST.get () in
+  B.popped_modifies h1 h11;
+  let loc = B.loc_region_only false (HS.get_tip h1) in
+  _lemma_nodelist_contained_in_unmodified_mem h1 h11 loc (as_list h11 d1);
+  _lemma_nodelist_contained_in_unmodified_mem h1 h11 loc (as_list h11 d2);
+  _lemma_nodelist_conn_in_unmodified_mem h1 h11 loc (as_list h11 d1);
+  _lemma_nodelist_conn_in_unmodified_mem h1 h11 loc (as_list h11 d2);
+  admit () (* Due to recent "double ghost" change *)
+
+#reset-options
+
+/// Automatic validity maintenance
+///
+/// These are lemmas that you shouldn't really need to refer to
+/// manually. If you do, it is (likely) a bug wrt the patterns, and
+/// you should ask someone who knows about how this library works to
+/// look at things.
+
+let auto_dll_remains_valid_upon_staying_unchanged h0 h1 l d =
+  _lemma_nodelist_contained_in_unmodified_mem h0 h1 l (as_list h1 d);
+  _lemma_nodelist_conn_in_unmodified_mem h0 h1 l (as_list h1 d)
+
+let auto_node_remains_valid_upon_staying_unchanged h0 h1 l n = ()
+
+let auto_node_remains_unchanged_upon_staying_unchanged_val h0 h1 n = ()
+
+/// Automatic footprint maintenance
+///
+/// These are lemmas that you shouldn't really need to refer to
+/// manually. If you do, it is (likely) a bug wrt the patterns, and
+/// you should ask someone who knows about how this library works to
+/// look at things.
+
+let auto_dll_fp_upon_staying_unchanged h0 h1 l d = ()
+
+/// Automatic value maintenance
+///
+/// These are lemmas that you shouldn't really need to refer to
+/// manually. If you do, it is (likely) a bug wrt the patterns, and
+/// you should ask someone who knows about how this library works to
+/// look at things.
+
+let auto_dll_as_list_staying_unchanged h0 h1 l d =()
+
+let auto_dll_as_payload_list_staying_unchanged h0 h1 loc d =
+  let rec aux loc nl : Lemma
+      (requires (
+          B.modifies loc h0 h1 /\
+          DLL.nodelist_contained h0 nl /\
+          B.loc_disjoint (DLL.nodelist_fp0 nl) loc))
+      (ensures (g_node_vals h0 nl == g_node_vals h1 nl)) =
+    match nl with
+    | [] -> ()
+    | hd :: tl -> aux loc tl in
+  aux loc (as_list h1 d)
+
+let auto_node_val_staying_unchanged h0 h1 l n = ()
+
+/// Properties of nodes inside and outside lists
+///
+/// These are lemmas that you shouldn't really need to refer to
+/// manually. If you do, it is (likely) a bug wrt the patterns, and
+/// you should ask someone who knows about how this library works to
+/// look at things.
+
+let auto_node_in_list_is_included h0 n d =
+  _lemma_node_in_list_is_included n (as_list h0 d)
+
+let auto_node_in_list_is_valid h0 n d =
+  DLL.extract_nodelist_contained h0 (as_list h0 d) (as_list h0 d `L.index_of` n)
+
+/// Properties related to unchanged connections
+///
+/// These are lemmas that you shouldn't really need to refer to
+/// manually. If you do, it is (likely) a bug wrt the patterns, and
+/// you should ask someone who knows about how this library works to
+/// look at things.
+
+let auto_unchanged_node_connections_list_unchanged h0 h1 d n =
+  assert (B.loc_disjoint (B.loc_buffer d) (DLL.dll_fp0 (d@h0)));
+  DLL.extract_nodelist_fp0 (as_list h0 d) (as_list h0 d `L.index_of` n);
+  assert (B.loc_disjoint (B.loc_buffer d) (B.loc_buffer n))
+
+#set-options "--z3rlimit 10"
+
+let auto_unchanged_node_connections_dll_valid h0 h1 d (n:node 'a) =
+  DLL.extract_nodelist_fp0 (as_list h0 d) (as_list h0 d `L.index_of` n);
+  assert (d@h0 == d@h1);
+  assert (as_list h0 d == as_list h1 d);
+  let rec aux1 #nl' (nl:list (node 'a)) :
+    Lemma
+      (requires (
+          (B.modifies (B.loc_buffer n) h0 h1) /\
+          (DLL.nodelist_contained h0 nl) /\
+          (DLL.nodelist_aa_r nl) /\
+          (nl' `L.append` nl == as_list h1 d) /\
+          (n `L.memP` nl \/ B.loc_buffer n `B.loc_disjoint` DLL.nodelist_fp0 nl)))
+      (ensures (DLL.nodelist_contained h1 nl))
+      (decreases (L.length nl)) =
+    match nl with
+    | [] -> ()
+    | x :: xs ->
+      let nl1', nl1 = L.snoc (nl', x), xs in
+      L.append_l_cons x xs nl';
+      aux1 #nl1' nl1 in
+  aux1 #[] (as_list h1 d);
+  assert (DLL.nodelist_contained h1 (as_list h1 d));
+  assert ((d@h1).DLL.lhead =!= B.null);
+  assert ((d@h1).DLL.ltail =!= B.null);
+  let rec aux2 #nl' (nl:list (node 'a)) :
+    Lemma
+      (requires (
+          (B.modifies (B.loc_buffer n) h0 h1) /\
+          unchanged_node_connections h0 h1 n /\
+          (DLL.nodelist_contained h0 nl) /\
+          (DLL.nodelist_contained h1 nl) /\
+          (DLL.nodelist_conn h0 nl) /\
+          (DLL.nodelist_aa_r nl) /\
+          (nl' `L.append` nl == as_list h1 d) /\
+          (n `L.memP` nl \/ B.loc_buffer n `B.loc_disjoint` DLL.nodelist_fp0 nl)))
+      (ensures (DLL.nodelist_conn h1 nl))
+      (decreases (L.length nl)) =
+    match nl with
+    | [] -> ()
+    | n1 :: rest ->
+      match rest with
+      | [] -> ()
+      | n2 :: ns ->
+        let nl1', nl1 = L.snoc (nl', n1), rest in
+        L.append_l_cons n1 rest nl';
+        aux2 #nl1' nl1;
+        assert (DLL.nodelist_conn h1 rest);
+        FStar.Classical.arrow_to_impl #(n `L.memP` rest) #((n1@h1).DLL.flink == (n1@h0).DLL.flink)
+          (fun _ -> DLL.extract_nodelist_fp0 rest (rest `L.index_of` n));
+        FStar.Classical.arrow_to_impl #(n `L.memP` ns) #((n2@h1).DLL.blink == (n2@h0).DLL.blink)
+          (fun _ -> DLL.extract_nodelist_fp0 ns (ns `L.index_of` n)) in
+  aux2 #[] (as_list h1 d);
+  assert (DLL.nodelist_conn h1 (as_list h1 d));
+  FStar.Classical.arrow_to_impl
+  #((d@h1).DLL.lhead =!= n) #(((d@h1).DLL.lhead@h1).DLL.blink == B.null)
+    (fun _ ->
+       let l = L.tl (as_list h1 d) in
+       DLL.extract_nodelist_fp0 l (l `L.index_of` n));
+  L.lemma_unsnoc_is_last (as_list h1 d);
+  FStar.Classical.arrow_to_impl
+  #((d@h1).DLL.ltail =!= n) #(((d@h1).DLL.ltail@h1).DLL.flink == B.null)
+    (fun _ ->
+       let l, _ = L.unsnoc (as_list h1 d) in
+       let i = as_list h1 d `L.index_of` n in
+       assert (i < L.length (as_list h1 d));
+       assert (i = L.length (as_list h1 d) ==> (d@h1).DLL.ltail == n);
+       assert ((d@h1).DLL.ltail =!= n);
+       assert (i < L.length (as_list h1 d) - 1);
+       L.lemma_unsnoc_length (as_list h1 d);
+       L.lemma_unsnoc_index (as_list h1 d) i;
+       DLL.extract_nodelist_fp0 l (l `L.index_of` n))
+
+#reset-options
+
+/// Properties related to pushes and pops
+///
+/// These are lemmas that you shouldn't really need to refer to
+/// manually. If you do, it is (likely) a bug wrt the patterns, and
+/// you should ask someone who knows about how this library works to
+/// look at things.
+
+let auto_dll_push_pop h0 h1 h2 h3 d = ()
+
+let auto_dll_fp_push_pop h0 h1 h2 h3 d = ()
+
+let auto_dll_fp_disjoint_push h0 h1 d = ()
