examples/doublylinkedlist/DoublyLinkedListIface.fsti
@@ -1,0 +1,521 @@
+(*
+   Copyright 2008-2019 Microsoft Research
+
+   Licensed under the Apache License, Version 2.0 (the "License");
+   you may not use this file except in compliance with the License.
+   You may obtain a copy of the License at
+
+       http://www.apache.org/licenses/LICENSE-2.0
+
+   Unless required by applicable law or agreed to in writing, software
+   distributed under the License is distributed on an "AS IS" BASIS,
+   WITHOUT WARRANTIES OR CONDITIONS OF ANY KIND, either express or implied.
+   See the License for the specific language governing permissions and
+   limitations under the License.
+*)
+
+module DoublyLinkedListIface
+
+module HS = FStar.HyperStack
+module HST = FStar.HyperStack.ST
+module L = FStar.List.Tot
+module B = LowStar.Buffer
+
+/// Abstract types defined by this library
+
+(** A singular node which stores a value of type [a] *)
+val node (a:Type0) : Type0
+
+(** A doublylinkedlist of elements of type [a] *)
+val dll (a:Type0) : Type0
+
+/// Abstract Validity Predicates
+
+val node_valid (h:HS.mem) (n:node 'a) : prop
+
+val dll_valid (h:HS.mem) (d:dll 'a) : prop
+
+/// Abstract node and list footprints
+
+val fp_node (n:node 'a) : GTot B.loc
+
+val fp_dll (h:HS.mem) (d:dll 'a) : GTot B.loc
+
+/// Getters and setters for [node]s
+
+val g_node_val (h:HS.mem) (n:node 'a) : GTot 'a
+
+val node_val (n:node 'a) :
+  HST.StackInline 'a
+    (requires (fun h0 -> node_valid h0 n))
+    (ensures (fun h0 v h1 -> h0 == h1 /\ v == g_node_val h0 n))
+
+val node_of (v:'a) :
+  HST.StackInline (node 'a)
+    (requires (fun h0 -> True))
+    (ensures (fun h0 n h1 ->
+         B.modifies B.loc_none h0 h1 /\
+         B.fresh_loc (fp_node n) h0 h1 /\
+         node_valid h1 n /\
+         v == g_node_val h1 n))
+
+/// Abstract Predicate to help "recall" that updating the payload
+/// leaves connections unchanged
+
+val unchanged_node_connections (h0 h1:HS.mem) (n:node 'a) : GTot prop
+
+/// Be able to modify the payload of a node easily, without affecting
+/// membership
+
+val node_update (n:node 'a) (v:'a) :
+  HST.StackInline (unit)
+    (requires (fun h0 -> node_valid h0 n))
+    (ensures (fun h0 () h1 ->
+         B.modifies (fp_node n) h0 h1 /\
+         node_valid h1 n /\
+         v == g_node_val h1 n /\
+         unchanged_node_connections h0 h1 n))
+
+/// Viewing ghostly state of a DoublyLinkedList as a list of nodes,
+/// and as list of payloads
+
+val as_list (h:HS.mem) (d:dll 'a) : GTot (list (node 'a))
+
+let rec g_node_vals (h:HS.mem) (l:list (node 'a)) : GTot (list 'a) =
+  match l with
+  | [] -> []
+  | hd :: tl -> g_node_val h hd :: g_node_vals h tl
+
+let as_payload_list (h:HS.mem) (d:dll 'a) : GTot (list 'a) =
+  g_node_vals h (as_list h d)
+
+/// Creating an empty DoublyLinkedList, and quickly accessing the head
+/// and tail of a DoublyLinkedList
+
+val dll_new (u:unit)  :
+  HST.StackInline (dll 'a)
+    (requires (fun h0 -> True))
+    (ensures (fun h0 d h1 ->
+         B.modifies B.loc_none h0 h1 /\
+         B.fresh_loc (fp_dll h1 d) h0 h1 /\
+         dll_valid h1 d /\
+         as_list h1 d == []))
+
+val is_empty (d:dll 'a) :
+  HST.StackInline (bool)
+    (requires (fun h0 -> dll_valid h0 d))
+    (ensures (fun h0 y h1 ->
+         (h0 == h1) /\
+         (y <==> as_list h0 d == [])))
+
+val dll_head (d:dll 'a) :
+  HST.StackInline (node 'a)
+    (requires (fun h0 -> dll_valid h0 d /\ L.length (as_list h0 d) > 0))
+    (ensures (fun h0 n h1 ->
+         B.modifies B.loc_none h0 h1 /\
+         dll_valid h1 d /\
+         node_valid h1 n /\
+         as_list h0 d == as_list h1 d /\
+         n == L.hd (as_list h0 d)))
+
+val dll_tail (d:dll 'a) :
+  HST.StackInline (node 'a)
+    (requires (fun h0 -> dll_valid h0 d /\ L.length (as_list h0 d) > 0))
+    (ensures (fun h0 n h1 ->
+         h0 == h1 /\
+         dll_valid h1 d /\
+         node_valid h1 n /\
+         as_list h0 d == as_list h1 d /\
+         n == snd (L.unsnoc (as_list h0 d))))
+
+/// Moving forwards or backwards in a list
+
+val has_next (d:dll 'a) (n:node 'a) :
+  HST.StackInline bool
+    (requires (fun h0 ->
+         dll_valid h0 d /\
+         node_valid h0 n /\
+         n `L.memP` as_list h0 d))
+    (ensures (fun h0 y h1 ->
+         (h0 == h1) /\
+         (y <==> L.index_of (as_list h0 d) n < L.length (as_list h0 d) - 1)))
+
+val has_prev (d:dll 'a) (n:node 'a) :
+  HST.StackInline bool
+    (requires (fun h0 ->
+         dll_valid h0 d /\
+         node_valid h0 n /\
+         n `L.memP` as_list h0 d))
+    (ensures (fun h0 y h1 ->
+         (h0 == h1) /\
+         (y <==> L.index_of (as_list h0 d) n > 0)))
+
+val next_node (d:dll 'a) (n:node 'a) :
+  HST.StackInline (node 'a)
+    (requires (fun h0 ->
+         dll_valid h0 d /\
+         n `L.memP` as_list h0 d /\
+         L.index_of (as_list h0 d) n < L.length (as_list h0 d) - 1))
+    (ensures (fun h0 n' h1 ->
+         h0 == h1 /\
+         dll_valid h1 d /\
+         node_valid h1 n /\
+         as_list h0 d == as_list h1 d /\
+         n' == L.index (as_list h0 d) (L.index_of (as_list h0 d) n + 1)))
+
+val prev_node (d:dll 'a) (n:node 'a) :
+  HST.StackInline (node 'a)
+    (requires (fun h0 ->
+         dll_valid h0 d /\
+         n `L.memP` as_list h0 d /\
+         L.index_of (as_list h0 d) n > 0))
+    (ensures (fun h0 n' h1 ->
+         h0 == h1 /\
+         dll_valid h1 d /\
+         node_valid h1 n /\
+         as_list h0 d == as_list h1 d /\
+         n' == L.index (as_list h0 d) (L.index_of (as_list h0 d) n - 1)))
+
+/// DoublyLinkedList operations on standard [list]s instead
+
+let l_insert_at_head (l:list 'a) (x:'a) : GTot (list 'a) =
+  x :: l
+
+let l_insert_at_tail (l:list 'a) (x:'a) : GTot (list 'a) =
+  L.snoc (l, x)
+
+let l_insert_before (x0:'a) (l:list 'a{x0 `L.memP` l}) (x:'a) : GTot (list 'a) =
+  let l1, l2 = L.split_using l x0 in
+  l1 `L.append` (x :: l2)
+
+let l_insert_before' (i:nat) (l:list 'a) (x:'a) : GTot (list 'a) =
+  let l1, l2 = L.splitAt i l in
+  l1 `L.append` (x :: l2)
+
+let l_insert_after (x0:'a) (l:list 'a{x0 `L.memP` l}) (x:'a) : GTot (list 'a) =
+  let l1, x1 :: l2 = L.lemma_split_using l x0; L.split_using l x0 in
+  assert (x0 == x1);
+  l1 `L.append` (x0 :: (x :: l2))
+
+let l_insert_after' (i:nat) (l:list 'a{i < L.length l}) (x:'a) : GTot (list 'a) =
+  let l1, x1 :: l2 = L.lemma_splitAt_snd_length i l; L.splitAt i l in
+  l1 `L.append` ((L.index l i) :: (x :: l2))
+
+let l_remove_head (l:list 'a{L.length l > 0}) : GTot (list 'a) =
+  match l with
+  | _ :: l' -> l'
+
+let l_remove_tail (l:list 'a{L.length l > 0}) : GTot (list 'a) =
+  let l', _ = L.unsnoc l in
+  l'
+
+let l_remove_mid (l:list 'a{L.length l > 0}) (x:'a {x `L.memP` l}) : GTot (list 'a) =
+  let l1, x0 :: l2 = L.lemma_split_using l x; L.split_using l x in
+  assert (x == x0);
+  l1 `L.append` l2
+
+let l_remove_mid' (l:list 'a{L.length l > 0}) (i:nat{i < L.length l}) : GTot (list 'a) =
+  let l1, x0 :: l2 = L.lemma_splitAt_snd_length i l; L.splitAt i l in
+  l1 `L.append` l2
+
+let l_append (l1 l2:list 'a) : GTot (list 'a) =
+  l1 `L.append` l2
+
+let l_split_using (l:list 'a) (x:'a{x `L.memP` l}) : GTot (list 'a * list 'a) =
+  L.split_using l x
+
+let l_split_using' (l:list 'a) (i:nat) : GTot (list 'a * list 'a) =
+  L.splitAt i l
+
+/// Useful "shortform" for equivalence of [loc]s
+
+let loc_equiv (a b:B.loc) =
+  B.loc_includes a b /\ B.loc_includes b a
+
+/// Stateful DoublyLinkedList operations
+///
+/// These are most likely what you want to be using when writing
+/// code. The rest of this interface lets you talk about these
+/// operations easily.
+
+val dll_insert_at_head (#t:Type0) (d:dll t) (n:node t) :
+  HST.Stack unit
+    (requires (fun h0 -> dll_valid h0 d /\ node_valid h0 n /\ (fp_node n `B.loc_disjoint` fp_dll h0 d)))
+    (ensures (fun h0 () h1 ->
+         B.modifies (fp_dll h1 d) h0 h1 /\
+         fp_dll h1 d `loc_equiv` B.loc_union (fp_dll h0 d) (fp_node n) /\
+         dll_valid h1 d /\ node_valid h1 n /\
+         as_payload_list h1 d == l_insert_at_head (as_payload_list h0 d) (g_node_val h0 n) /\
+         as_list h1 d == l_insert_at_head (as_list h0 d) n))
+
+val dll_insert_at_tail (#t:Type0) (d:dll t) (n:node t) :
+  HST.Stack unit
+    (requires (fun h0 -> dll_valid h0 d /\ node_valid h0 n /\ (fp_node n `B.loc_disjoint` fp_dll h0 d)))
+    (ensures (fun h0 () h1 ->
+         B.modifies (fp_dll h1 d) h0 h1 /\
+         fp_dll h1 d `loc_equiv` B.loc_union (fp_dll h0 d) (fp_node n) /\
+         dll_valid h1 d /\ node_valid h1 n /\
+         as_payload_list h1 d == l_insert_at_tail (as_payload_list h0 d) (g_node_val h0 n) /\
+         as_list h1 d == l_insert_at_tail (as_list h0 d) n))
+
+val dll_insert_before (#t:Type0) (n':node t) (d:dll t) (n:node t) :
+  HST.Stack unit
+    (requires (fun h0 -> dll_valid h0 d /\ node_valid h0 n /\ (fp_node n `B.loc_disjoint` fp_dll h0 d) /\ n' `L.memP` as_list h0 d))
+    (ensures (fun h0 () h1 ->
+         B.modifies (fp_dll h1 d) h0 h1 /\
+         fp_dll h1 d `loc_equiv` B.loc_union (fp_dll h0 d) (fp_node n) /\
+         dll_valid h1 d /\ node_valid h1 n /\
+         as_payload_list h1 d == l_insert_before'
+           (as_list h0 d `L.index_of` n') (as_payload_list h0 d) (g_node_val h0 n) /\
+         as_list h1 d == l_insert_before n' (as_list h0 d) n))
+
+val dll_insert_after (#t:Type0) (n':node t) (d:dll t) (n:node t) :
+  HST.Stack unit
+    (requires (fun h0 -> dll_valid h0 d /\ node_valid h0 n /\ (fp_node n `B.loc_disjoint` fp_dll h0 d) /\ n' `L.memP` as_list h0 d))
+    (ensures (fun h0 () h1 ->
+         B.modifies (fp_dll h1 d) h0 h1 /\
+         fp_dll h1 d `loc_equiv` B.loc_union (fp_dll h0 d) (fp_node n) /\
+         dll_valid h1 d /\ node_valid h1 n /\
+         L.length (as_payload_list h0 d) = L.length (as_list h0 d) /\ // TODO: Why?!
+         as_payload_list h1 d == l_insert_after'
+           (as_list h0 d `L.index_of` n') (as_payload_list h0 d) (g_node_val h0 n) /\
+         as_list h1 d == l_insert_after n' (as_list h0 d) n))
+
+unfold
+let fp_strictly_disjoint_union (l l1 l2:B.loc) =
+  l `loc_equiv` B.loc_union l1 l2 /\
+  l1 `B.loc_disjoint` l2
+
+unfold
+let aux_fp_split_by_node (h0 h1:HS.mem) (d:dll 'a) (n:node 'a) =
+  fp_strictly_disjoint_union (fp_dll h0 d) (fp_dll h1 d) (fp_node n)
+
+val dll_remove_head (#t:Type0) (d:dll t) :
+  HST.Stack unit
+    (requires (fun h0 -> dll_valid h0 d /\ L.length (as_list h0 d) > 0))
+    (ensures (fun h0 () h1 ->
+         B.modifies (fp_dll h0 d) h0 h1 /\
+         aux_fp_split_by_node h0 h1 d (L.hd (as_list h0 d)) /\
+         dll_valid h1 d /\
+         node_valid h1 (L.hd (as_list h0 d)) /\
+         g_node_val h0 (L.hd (as_list h0 d)) == g_node_val h1 (L.hd (as_list h0 d)) /\
+         as_payload_list h1 d == l_remove_head (as_payload_list h0 d) /\
+         as_list h1 d == l_remove_head (as_list h0 d)))
+
+val dll_remove_tail (#t:Type0) (d:dll t) :
+  HST.Stack unit
+    (requires (fun h0 -> dll_valid h0 d /\ L.length (as_list h0 d) > 0))
+    (ensures (fun h0 () h1 ->
+         B.modifies (fp_dll h0 d) h0 h1 /\
+         aux_fp_split_by_node h0 h1 d (L.last (as_list h0 d)) /\
+         dll_valid h1 d /\
+         node_valid h1 (L.last (as_list h0 d)) /\
+         g_node_val h0 (L.last (as_list h0 d)) == g_node_val h1 (L.last (as_list h0 d)) /\
+         as_payload_list h1 d == l_remove_tail (as_payload_list h0 d) /\
+         as_list h1 d == l_remove_tail (as_list h0 d)))
+
+val dll_remove_mid (#t:Type0) (d:dll t) (n:node t) :
+  HST.Stack unit
+    (requires (fun h0 -> dll_valid h0 d /\ n `L.memP` as_list h0 d))
+    (ensures (fun h0 () h1 ->
+         B.modifies (fp_dll h0 d) h0 h1 /\
+         aux_fp_split_by_node h0 h1 d n /\
+         dll_valid h1 d /\
+         g_node_val h0 n == g_node_val h1 n /\
+         L.length (as_payload_list h0 d) = L.length (as_list h0 d) /\ // TODO: Why?!
+         as_payload_list h1 d == l_remove_mid' (as_payload_list h0 d) (as_list h0 d `L.index_of` n) /\
+         as_list h1 d == l_remove_mid (as_list h0 d) n))
+
+val dll_append (#t:Type0) (d1 d2:dll t) :
+  HST.Stack unit
+    (requires (fun h0 ->
+         dll_valid h0 d1 /\
+         dll_valid h0 d2 /\
+         fp_dll h0 d1 `B.loc_disjoint` fp_dll h0 d2))
+    (ensures (fun h0 () h1 ->
+         B.modifies (fp_dll h0 d1 `B.loc_union` fp_dll h0 d2) h0 h1 /\
+         fp_strictly_disjoint_union (B.loc_union (fp_dll h1 d1) (fp_dll h1 d2))
+           (fp_dll h0 d1) (fp_dll h0 d2) /\
+         dll_valid h1 d1 /\
+         as_payload_list h1 d1 == as_payload_list h0 d1 `l_append` as_payload_list h0 d2 /\
+         as_list h1 d1 == as_list h0 d1 `l_append` as_list h0 d2))
+
+val dll_split_using (#t:Type0) (d1 d2:dll t) (n:node t) :
+  HST.Stack unit
+    (requires (fun h0 ->
+         dll_valid h0 d1 /\
+         n `L.memP` as_list h0 d1 /\
+         dll_valid h0 d2 /\
+         fp_dll h0 d1 `B.loc_disjoint` fp_dll h0 d2 /\
+         as_list h0 d2 == []))
+    (ensures (fun h0 () h1 ->
+         B.modifies (fp_dll h0 d1 `B.loc_union` fp_dll h0 d2) h0 h1 /\
+         fp_strictly_disjoint_union (B.loc_union (fp_dll h1 d1) (fp_dll h1 d2))
+           (fp_dll h0 d1) (fp_dll h0 d2) /\
+         dll_valid h1 d1 /\
+         dll_valid h1 d2 /\
+         (as_payload_list h1 d1, as_payload_list h1 d2) == l_split_using' (as_payload_list h0 d1) (as_list h0 d1 `L.index_of` n) /\
+         (as_list h1 d1, as_list h1 d2) == l_split_using (as_list h0 d1) n))
+
+/// Automatic validity maintenance
+///
+/// These are lemmas that you shouldn't really need to refer to
+/// manually. If you do, it is (likely) a bug wrt the patterns, and
+/// you should ask someone who knows about how this library works to
+/// look at things.
+
+val auto_dll_remains_valid_upon_staying_unchanged (h0 h1:HS.mem) (l:B.loc) (d:dll 'a) :
+  Lemma
+    (requires (dll_valid h0 d /\
+               B.modifies l h0 h1 /\
+               B.loc_disjoint (fp_dll h0 d) l))
+    (ensures (dll_valid h1 d))
+    [SMTPat (dll_valid h1 d); SMTPat (B.modifies l h0 h1)]
+
+val auto_node_remains_valid_upon_staying_unchanged (h0 h1:HS.mem) (l:B.loc) (n:node 'a) :
+  Lemma
+    (requires (node_valid h0 n /\
+               B.modifies l h0 h1 /\
+               B.loc_disjoint (fp_node n) l))
+    (ensures (node_valid h1 n))
+    [SMTPat (node_valid h1 n); SMTPat (B.modifies l h0 h1)]
+
+/// Automatic footprint maintenance
+///
+/// These are lemmas that you shouldn't really need to refer to
+/// manually. If you do, it is (likely) a bug wrt the patterns, and
+/// you should ask someone who knows about how this library works to
+/// look at things.
+
+val auto_dll_fp_upon_staying_unchanged (h0 h1:HS.mem) (l:B.loc) (d:dll 'a) :
+  Lemma
+    (requires (dll_valid h0 d /\
+               B.modifies l h0 h1 /\
+               B.loc_disjoint (fp_dll h0 d) l))
+    (ensures (fp_dll h1 d == fp_dll h0 d))
+    [SMTPat (fp_dll h1 d); SMTPat (B.modifies l h0 h1)]
+
+/// Automatic value maintenance
+///
+/// These are lemmas that you shouldn't really need to refer to
+/// manually. If you do, it is (likely) a bug wrt the patterns, and
+/// you should ask someone who knows about how this library works to
+/// look at things.
+
+val auto_dll_as_list_staying_unchanged (h0 h1:HS.mem) (l:B.loc) (d:dll 'a) :
+  Lemma
+    (requires (dll_valid h0 d /\
+               B.modifies l h0 h1 /\
+               B.loc_disjoint (fp_dll h0 d) l))
+    (ensures (as_list h1 d == as_list h0 d))
+    [SMTPat (as_list h1 d); SMTPat (B.modifies l h0 h1)]
+
+val auto_dll_as_payload_list_staying_unchanged (h0 h1:HS.mem) (l:B.loc) (d:dll 'a) :
+  Lemma
+    (requires (dll_valid h0 d /\
+               B.modifies l h0 h1 /\
+               B.loc_disjoint (fp_dll h0 d) l))
+    (ensures (as_payload_list h1 d == as_payload_list h0 d))
+    [SMTPat (as_payload_list h1 d); SMTPat (B.modifies l h0 h1)]
+
+val auto_node_val_staying_unchanged (h0 h1:HS.mem) (l:B.loc) (n:node 'a) :
+  Lemma
+    (requires (node_valid h0 n /\
+               B.modifies l h0 h1 /\
+               B.loc_disjoint (fp_node n) l))
+    (ensures (g_node_val h1 n == g_node_val h0 n))
+    [SMTPat (g_node_val h1 n); SMTPat (B.modifies l h0 h1)]
+
+/// Properties of nodes inside and outside lists
+///
+/// These are lemmas that you shouldn't really need to refer to
+/// manually. If you do, it is (likely) a bug wrt the patterns, and
+/// you should ask someone who knows about how this library works to
+/// look at things.
+
+val auto_node_in_list_is_included (h0:HS.mem) (n:node 'a) (d:dll 'a) :
+  Lemma
+    (requires (dll_valid h0 d /\
+               n `L.memP` as_list h0 d))
+    (ensures (B.loc_includes (fp_dll h0 d) (fp_node n)))
+    [SMTPat (B.loc_includes (fp_dll h0 d) (fp_node n))]
+
+val auto_node_in_list_is_valid (h0:HS.mem) (n:node 'a) (d:dll 'a) :
+  Lemma
+    (requires (dll_valid h0 d /\
+               n `L.memP` as_list h0 d))
+    (ensures (node_valid h0 n))
+    [SMTPat (node_valid h0 n);
+     SMTPat (dll_valid h0 d)]
+
+/// Properties related to unchanged connections
+///
+/// These are lemmas that you shouldn't really need to refer to
+/// manually. If you do, it is (likely) a bug wrt the patterns, and
+/// you should ask someone who knows about how this library works to
+/// look at things.
+
+val auto_unchanged_node_connections_list_unchanged (h0 h1:HS.mem) (d:dll 'a) (n:node 'a) :
+  Lemma
+    (requires (dll_valid h0 d /\
+               n `L.memP` as_list h0 d /\
+               B.modifies (fp_node n) h0 h1 /\
+               unchanged_node_connections h0 h1 n))
+    (ensures (as_list h1 d == as_list h0 d))
+    [SMTPat (as_list h1 d);
+     SMTPat (B.modifies (fp_node n) h0 h1);
+     SMTPat (unchanged_node_connections h0 h1 n)]
+
+val auto_unchanged_node_connections_dll_valid (h0 h1:HS.mem) (d:dll 'a) (n:node 'a) :
+  Lemma
+    (requires (dll_valid h0 d /\
+               n `L.memP` as_list h0 d /\
+               B.modifies (fp_node n) h0 h1 /\
+               unchanged_node_connections h0 h1 n))
+    (ensures (dll_valid h1 d))
+    [SMTPat (dll_valid h1 d);
+     SMTPat (B.modifies (fp_node n) h0 h1);
+     SMTPat (unchanged_node_connections h0 h1 n)]
+
+/// Properties related to pushes and pops
+///
+/// These are lemmas that you shouldn't really need to refer to
+/// manually. If you do, it is (likely) a bug wrt the patterns, and
+/// you should ask someone who knows about how this library works to
+/// look at things.
+
+val auto_dll_push_pop (h0 h1 h2 h3:HS.mem) (d:dll 'a) :
+  Lemma
+    (requires (
+        HS.fresh_frame h0 h1 /\
+        B.loc_disjoint (fp_dll h2 d) (B.loc_region_only false (HS.get_tip h2)) /\
+        HS.get_tip h1 == HS.get_tip h2 /\
+        dll_valid h2 d /\
+        HS.popped h2 h3))
+    (ensures (dll_valid h3 d))
+    [SMTPat (dll_valid h3 d);
+     SMTPat (HS.fresh_frame h0 h1);
+     SMTPat (HS.popped h2 h3)]
+
+val auto_dll_fp_push_pop (h0 h1 h2 h3:HS.mem) (d:dll 'a) :
+  Lemma
+    (requires (
+        HS.fresh_frame h0 h1 /\
+        B.loc_disjoint (fp_dll h2 d) (B.loc_region_only false (HS.get_tip h2)) /\
+        HS.get_tip h1 == HS.get_tip h2 /\
+        dll_valid h2 d /\
+        HS.popped h2 h3))
+    (ensures (fp_dll h3 d == fp_dll h2 d))
+    [SMTPat (fp_dll h3 d);
+     SMTPat (HS.fresh_frame h0 h1);
+     SMTPat (HS.popped h2 h3)]
+
+val auto_dll_fp_disjoint_push (h0 h1:HS.mem) (d:dll 'a) :
+  Lemma
+    (requires (
+        HS.fresh_frame h0 h1 /\
+        dll_valid h0 d))
+    (ensures (
+        B.loc_disjoint (fp_dll h1 d) (B.loc_region_only false (HS.get_tip h1))))
+    [SMTPat (B.loc_disjoint (fp_dll h1 d) (B.loc_region_only false (HS.get_tip h1)));
+     SMTPat (HS.fresh_frame h0 h1)]
